Migrate time/geom1d changes from Phys and add new geom3d file

expressions/geom1d_expr.lean
@@ -16,14 +16,14 @@ structure geom1d_frame_var extends var
 
 
 inductive geom1d_frame_expr : Type 1 --{f : fm scalar T}
-| lit (f : fm scalar LENGTH) : geom1d_frame_expr
+| lit (f : geom1d_frame) : geom1d_frame_expr
 | var (v : geom1d_frame_var) : geom1d_frame_expr
 
 
 abbreviation geom1d_frame_env :=
-  geom1d_frame_var → fm scalar LENGTH
+  geom1d_frame_var → geom1d_frame
 abbreviation geom1d_frame_eval :=
-  geom1d_frame_env → geom1d_frame_expr → fm scalar LENGTH
+  geom1d_frame_env → geom1d_frame_expr → geom1d_frame
 
 def default_frame_env : geom1d_frame_env := 
   λv, geom1d_std_frame
@@ -38,38 +38,38 @@ def static_frame_eval : geom1d_frame_eval
 | env_ (geom1d_frame_expr.lit f) := f
 | env_ (geom1d_frame_expr.var v) := env_ v
 
-def geom1d_frame_expr.value (expr_ : geom1d_frame_expr) : fm scalar LENGTH :=
+def geom1d_frame_expr.value (expr_ : geom1d_frame_expr) : geom1d_frame :=
   (static_frame_eval) (default_frame_env) expr_
 
 structure geom1d_space_var (f : geom1d_frame_expr) extends var
 
 inductive geom1d_space_expr (f : geom1d_frame_expr) : Type 1
-| lit (sp : spc scalar f.value) : geom1d_space_expr
+| lit (sp : geom1d_space f.value) : geom1d_space_expr
 | var (v : geom1d_space_var f) : geom1d_space_expr
 | mk : geom1d_space_expr
 
 abbreviation geom1d_space_env := Π(f : geom1d_frame_expr),
-  geom1d_space_var f → spc scalar f.value
+  geom1d_space_var f → geom1d_space f.value
 abbreviation geom1d_space_eval := Π(f : geom1d_frame_expr),
-  geom1d_space_env → geom1d_space_expr f → spc scalar f.value
+  geom1d_space_env → geom1d_space_expr f → geom1d_space f.value
 
 
 def default_space_env : geom1d_space_env := 
-  λf, λv, mk_space scalar f.value
+  λf, λv, mk_space f.value
 def default_space_eval : geom1d_space_eval := λf, λenv_, λexpr_, 
   begin
     cases expr_,
     exact expr_,
     exact (default_space_env f expr_),
-    exact mk_space scalar f.value
+    exact mk_space f.value
   end
 
 def static_space_eval : geom1d_space_eval 
 | f env_ (geom1d_space_expr.lit sp) := sp
 | f env_ (geom1d_space_expr.var v) := env_ f v
-| f env_ (geom1d_space_expr.mk) := mk_space scalar f.value
+| f env_ (geom1d_space_expr.mk) := mk_space f.value
 
-def geom1d_space_expr.value {f : geom1d_frame_expr} (expr_ : geom1d_space_expr f)  : spc scalar f.value :=
+def geom1d_space_expr.value {f : geom1d_frame_expr} (expr_ : geom1d_space_expr f)  : geom1d_space f.value :=
   (static_space_eval f) (default_space_env) expr_
 
 /-
@@ -79,12 +79,12 @@ structure transform_var
   {f1 : geom1d_frame_expr} (sp1 : geom1d_space_expr f1) {f2 : geom1d_frame_expr} (sp2 : geom1d_space_expr f2) extends var
 
 inductive geom1d_transform_expr
-  --{f1 : fm scalar LENGTH} {f2 : fm scalar LENGTH} (sp1 : spc scalar f1) (sp2:=sp1 : spc scalar f2) 
- -- (sp1 : Σf1 : fm scalar LENGTH, spc scalar f1)  (sp2 : Σf2 : fm scalar LENGTH, spc scalar f2 := sp1)
+  --{f1 : geom1d_frame} {f2 : geom1d_frame} (sp1 : geom1d_space f1) (sp2:=sp1 : geom1d_space f2) 
+ -- (sp1 : Σf1 : geom1d_frame, geom1d_space f1)  (sp2 : Σf2 : geom1d_frame, geom1d_space f2 := sp1)
   : Π {f1 : geom1d_frame_expr} (sp1 : geom1d_space_expr f1), Π {f2 : geom1d_frame_expr} (sp2 : geom1d_space_expr f2), Type 1
 | lit {f1 : geom1d_frame_expr} {sp1 : geom1d_space_expr f1} {f2 : geom1d_frame_expr} {sp2 : geom1d_space_expr f2} (p : geom1d_transform sp1.value sp2.value) : geom1d_transform_expr sp1 sp2
 | var {f1 : geom1d_frame_expr} {sp1 : geom1d_space_expr f1} {f2 : geom1d_frame_expr} {sp2 : geom1d_space_expr f2} (v : transform_var sp1 sp2) : geom1d_transform_expr sp1 sp2
-| compose_lit {f1 : geom1d_frame_expr} {sp1 : geom1d_space_expr f1} {f2 : fm scalar LENGTH} {sp2 : spc scalar f2} (t1 : geom1d_transform sp1.value sp2) 
+| compose_lit {f1 : geom1d_frame_expr} {sp1 : geom1d_space_expr f1} {f2 : geom1d_frame} {sp2 : geom1d_space f2} (t1 : geom1d_transform sp1.value sp2) 
   {f3 : geom1d_frame_expr} {sp3 : geom1d_space_expr f3}  (t2 : geom1d_transform sp2 sp3.value) : geom1d_transform_expr sp1 sp3
 | inv_lit {f1 : geom1d_frame_expr} {sp1 : geom1d_space_expr f1} {f2 : geom1d_frame_expr} {sp2 : geom1d_space_expr f2} (t : geom1d_transform sp2.value sp1.value) : geom1d_transform_expr sp1 sp2
 | compose 
@@ -116,8 +116,9 @@ abbreviation transform_eval
 
 
 def default_transform_env 
-  {f1 : geom1d_frame_expr} (sp1 : geom1d_space_expr f1) {f2 : geom1d_frame_expr} (sp2 : geom1d_space_expr f2) : transform_env sp1 sp2:=
-    λv, sp1.value.mk_geom1d_transform_to sp2.value
+  {f1 : geom1d_frame_expr} (sp1 : geom1d_space_expr f1) {f2 : geom1d_frame_expr} (sp2 : geom1d_space_expr f2) 
+    : transform_env sp1 sp2:=
+    λv, (sp1.value).mk_geom1d_transform_to sp2.value
 
 def default_transform_eval 
   {f1 : geom1d_frame_expr} (sp1 : geom1d_space_expr f1) {f2 : geom1d_frame_expr} (sp2 : geom1d_space_expr f2) : transform_eval sp1 sp2 :=
@@ -185,150 +186,150 @@ def geom1d_transform_expr.trans
 /-
 Duration
 -/
-structure displacement_var {f : geom1d_frame_expr} (sp : geom1d_space_expr f) extends var 
+structure displacement1d_var {f : geom1d_frame_expr} (sp : geom1d_space_expr f) extends var 
 
 /-
 Time
 -/
-structure position_var  {f : geom1d_frame_expr} (sp : geom1d_space_expr f) extends var
+structure position1d_var  {f : geom1d_frame_expr} (sp : geom1d_space_expr f) extends var
 set_option trace.app_builder true --need to fix scalar for this to work
 
-mutual inductive displacement_expr, position_expr {f : geom1d_frame_expr} (sp : geom1d_space_expr f)
-with displacement_expr : Type 1
-| zero : displacement_expr
-| one : displacement_expr 
-| lit (v : displacement sp.value) : displacement_expr
-| var (v : displacement_var sp) : displacement_expr
-| add_dur_dur (d1 : displacement_expr) (d2 : displacement_expr) : displacement_expr
-| neg_dur (d : displacement_expr) : displacement_expr
-| sub_dur_dur (d1 : displacement_expr) (d2 : displacement_expr) : displacement_expr
-| sub_position_position (t1 : position_expr) (t2 : position_expr) : displacement_expr
-| smul_dur (k : scalar_expr) (d : displacement_expr) : displacement_expr
-| apply_displacement_lit {f2 : geom1d_frame_expr} {sp2 : geom1d_space_expr f2} (v : geom1d_transform_expr sp2 sp) 
-    (d : displacement sp2.value) : displacement_expr
-with position_expr : Type 1
-| lit (p : position sp.value) : position_expr
-| var (v : position_var sp) : position_expr
-| add_dur_position (d : displacement_expr) (t : position_expr) : position_expr
-| apply_position_lit {f2 : geom1d_frame_expr} {sp2 : geom1d_space_expr f2} (v : geom1d_transform_expr sp2 sp) 
-    (t : position sp2.value) : position_expr
+mutual inductive displacement1d_expr, position1d_expr {f : geom1d_frame_expr} (sp : geom1d_space_expr f)
+with displacement1d_expr : Type 1
+| zero : displacement1d_expr
+| one : displacement1d_expr 
+| lit (v : displacement1d sp.value) : displacement1d_expr
+| var (v : displacement1d_var sp) : displacement1d_expr
+| add_dur_dur (d1 : displacement1d_expr) (d2 : displacement1d_expr) : displacement1d_expr
+| neg_dur (d : displacement1d_expr) : displacement1d_expr
+| sub_dur_dur (d1 : displacement1d_expr) (d2 : displacement1d_expr) : displacement1d_expr
+| sub_position1d_position1d (t1 : position1d_expr) (t2 : position1d_expr) : displacement1d_expr
+| smul_dur (k : scalar_expr) (d : displacement1d_expr) : displacement1d_expr
+| apply_displacement1d_lit {f2 : geom1d_frame_expr} {sp2 : geom1d_space_expr f2} (v : geom1d_transform_expr sp2 sp) 
+    (d : displacement1d sp2.value) : displacement1d_expr
+with position1d_expr : Type 1
+| lit (p : position1d sp.value) : position1d_expr
+| var (v : position1d_var sp) : position1d_expr
+| add_dur_position1d (d : displacement1d_expr) (t : position1d_expr) : position1d_expr
+| apply_position1d_lit {f2 : geom1d_frame_expr} {sp2 : geom1d_space_expr f2} (v : geom1d_transform_expr sp2 sp) 
+    (t : position1d sp2.value) : position1d_expr
 
 
-abbreviation displacement_env {f : geom1d_frame_expr} (sp : geom1d_space_expr f) := 
-  displacement_var sp → displacement sp.value
+abbreviation displacement1d_env {f : geom1d_frame_expr} (sp : geom1d_space_expr f) := 
+  displacement1d_var sp → displacement1d sp.value
 
 attribute [elab_as_eliminator] 
-abbreviation position_env {f : geom1d_frame_expr} (sp : geom1d_space_expr f) :=
-  position_var sp → position sp.value
+abbreviation position1d_env {f : geom1d_frame_expr} (sp : geom1d_space_expr f) :=
+  position1d_var sp → position1d sp.value
 
-abbreviation displacement_eval := Π{f : geom1d_frame_expr} (sp : geom1d_space_expr f),
-  position_env sp → displacement_env sp → displacement_expr sp → displacement sp.value
+abbreviation displacement1d_eval := Π{f : geom1d_frame_expr} (sp : geom1d_space_expr f),
+  position1d_env sp → displacement1d_env sp → displacement1d_expr sp → displacement1d sp.value
 
-abbreviation position_eval := Π{f : geom1d_frame_expr} (sp : geom1d_space_expr f), 
-  position_env sp → displacement_env sp → position_expr sp → position sp.value
+abbreviation position1d_eval := Π{f : geom1d_frame_expr} (sp : geom1d_space_expr f), 
+  position1d_env sp → displacement1d_env sp → position1d_expr sp → position1d sp.value
 
-def default_displacement_env {f : geom1d_frame_expr} (sp : geom1d_space_expr f) : displacement_env sp := λv, (mk_displacement sp.value 1)
-def default_displacement_eval : displacement_eval  
+def default_displacement1d_env {f : geom1d_frame_expr} (sp : geom1d_space_expr f) : displacement1d_env sp := λv, (mk_displacement1d sp.value 1)
+def default_displacement1d_eval : displacement1d_eval  
   := λf sp, λtenv_, λdenv_, λexpr_, 
   begin
     --cases expr_,
     --exact expr_,
-    --exact default_displacement_env sp expr_,
-    repeat {exact (mk_displacement sp.value 1)}
+    --exact default_displacement1d_env sp expr_,
+    repeat {exact (mk_displacement1d sp.value 1)}
   end
 
 --this needs to get fixed, perhaps eval should not depend on env but use a global one *shrug*
 --OR, a point evaluator needs to depend on a vector environment, and vice versa? may be acceptable
-def default_position_env {f : geom1d_frame_expr} (sp : geom1d_space_expr f) : position_env sp 
-  := (λv, (mk_position sp.value 1))
+def default_position1d_env {f : geom1d_frame_expr} (sp : geom1d_space_expr f) : position1d_env sp 
+  := (λv, (mk_position1d sp.value 1))
 
 
 set_option eqn_compiler.max_steps 8192
-mutual def static_displacement_eval, static_position_eval 
-with static_displacement_eval : displacement_eval 
-| f sp tenv_ denv_ (displacement_expr.zero) := 0
-| f sp tenv_ denv_ (displacement_expr.one) := mk_displacement sp.value 1
-| f sp tenv_ denv_ (displacement_expr.lit d) := d
-| f sp tenv_ denv_ (displacement_expr.var v) := denv_ v
-| f sp tenv_ denv_ (displacement_expr.add_dur_dur d1 d2) := (static_displacement_eval sp tenv_ denv_ d1) +ᵥ (static_displacement_eval sp tenv_ denv_ d2)
-| f sp tenv_ denv_ (displacement_expr.neg_dur d) := -(static_displacement_eval sp tenv_ denv_ d)
-| f sp tenv_ denv_ (displacement_expr.sub_dur_dur d1 d2) := (static_displacement_eval sp tenv_ denv_ d1) -ᵥ (static_displacement_eval sp tenv_ denv_ d2)
-| f sp tenv_ denv_ (displacement_expr.sub_position_position t1 t2) := (static_position_eval sp tenv_ denv_ t1) -ᵥ (static_position_eval sp tenv_ denv_ t2)
-| f sp tenv_ denv_ (displacement_expr.smul_dur s d) := (static_scalar_eval default_scalar_env s)•(static_displacement_eval sp tenv_ denv_ d)
-| f sp tenv_ denv_ (displacement_expr.apply_displacement_lit t d) := t.value.transform_displacement d
-with static_position_eval : position_eval
-| f sp tenv_ denv_ (position_expr.lit p) := p
-| f sp tenv_ denv_ (position_expr.var v) := tenv_ v
-| f sp tenv_ denv_ (position_expr.add_dur_position d t) := (static_displacement_eval sp tenv_ denv_ d) +ᵥ (static_position_eval sp tenv_ denv_ t)
-| f sp tenv_ denv_ (position_expr.apply_position_lit tr t) := tr.value.transform_position t
+mutual def static_displacement1d_eval, static_position1d_eval 
+with static_displacement1d_eval : displacement1d_eval 
+| f sp tenv_ denv_ (displacement1d_expr.zero) := 0
+| f sp tenv_ denv_ (displacement1d_expr.one) := mk_displacement1d sp.value 1
+| f sp tenv_ denv_ (displacement1d_expr.lit d) := d
+| f sp tenv_ denv_ (displacement1d_expr.var v) := denv_ v
+| f sp tenv_ denv_ (displacement1d_expr.add_dur_dur d1 d2) := (static_displacement1d_eval sp tenv_ denv_ d1) +ᵥ (static_displacement1d_eval sp tenv_ denv_ d2)
+| f sp tenv_ denv_ (displacement1d_expr.neg_dur d) := -(static_displacement1d_eval sp tenv_ denv_ d)
+| f sp tenv_ denv_ (displacement1d_expr.sub_dur_dur d1 d2) := (static_displacement1d_eval sp tenv_ denv_ d1) -ᵥ (static_displacement1d_eval sp tenv_ denv_ d2)
+| f sp tenv_ denv_ (displacement1d_expr.sub_position1d_position1d t1 t2) := (static_position1d_eval sp tenv_ denv_ t1) -ᵥ (static_position1d_eval sp tenv_ denv_ t2)
+| f sp tenv_ denv_ (displacement1d_expr.smul_dur s d) := (static_scalar_eval default_scalar_env s)•(static_displacement1d_eval sp tenv_ denv_ d)
+| f sp tenv_ denv_ (displacement1d_expr.apply_displacement1d_lit t d) := t.value.transform_displacement1d d
+with static_position1d_eval : position1d_eval
+| f sp tenv_ denv_ (position1d_expr.lit p) := p
+| f sp tenv_ denv_ (position1d_expr.var v) := tenv_ v
+| f sp tenv_ denv_ (position1d_expr.add_dur_position1d d t) := (static_displacement1d_eval sp tenv_ denv_ d) +ᵥ (static_position1d_eval sp tenv_ denv_ t)
+| f sp tenv_ denv_ (position1d_expr.apply_position1d_lit tr t) := tr.value.transform_position1d t
 
 
-def default_position_eval : position_eval := λf sp, λtenv_, λdenv_, λexpr_, 
+def default_position1d_eval : position1d_eval := λf sp, λtenv_, λdenv_, λexpr_, 
   begin
     cases expr_,
     exact expr_,
-    exact default_position_env sp expr_,
-    repeat {exact (mk_position sp.value 1)}
+    exact default_position1d_env sp expr_,
+    repeat {exact (mk_position1d sp.value 1)}
   end
 
-#check position_env
-#check default_position_env
+#check position1d_env
+#check default_position1d_env
 
-def position_expr.value {f : geom1d_frame_expr} {sp : geom1d_space_expr f} (expr_ : position_expr sp) : position sp.value :=
-  (static_position_eval sp) (default_position_env sp) (default_displacement_env sp) expr_
+def position1d_expr.value {f : geom1d_frame_expr} {sp : geom1d_space_expr f} (expr_ : position1d_expr sp) : position1d sp.value :=
+  (static_position1d_eval sp) (default_position1d_env sp) (default_displacement1d_env sp) expr_
 
-def displacement_expr.value {f : geom1d_frame_expr} {sp : geom1d_space_expr f} (expr_ : displacement_expr sp) : displacement sp.value :=
-  (static_displacement_eval sp) (default_position_env sp) (default_displacement_env sp) expr_
+def displacement1d_expr.value {f : geom1d_frame_expr} {sp : geom1d_space_expr f} (expr_ : displacement1d_expr sp) : displacement1d sp.value :=
+  (static_displacement1d_eval sp) (default_position1d_env sp) (default_displacement1d_env sp) expr_
 
 
 --not working -- lean doesn't play nice with notation and dependent types
 --notation `|`flit`|` := geom1d_frame_expr.lit flit
 --notation `|`slit`|` := geom1d_space_expr.lit slit
---instance {scalar : Type u} [field scalar] [inhabited scalar] {f : fm scalar LENGTH} {sp : spc scalar f} : has_coe (position sp) (position_expr sp) := ⟨λt, position_expr.lit t⟩
---instance {scalar : Type u} [field scalar] [inhabited scalar] {f : fm scalar LENGTH} {sp : spc scalar f} : has_coe (displacement sp) (displacement_expr sp) := ⟨λt, displacement_expr.lit t⟩
---instance {scalar : Type u} [field scalar] [inhabited scalar] : has_coe (fm scalar LENGTH) (geom1d_frame_expr scalar) := ⟨λf, geom1d_frame_expr.lit f⟩
---instance {scalar : Type u} [field scalar] [inhabited scalar] {f : fm scalar LENGTH} : has_coe (spc scalar f) (geom1d_space_expr scalar) := ⟨λs, geom1d_space_expr.lit s⟩
+--instance {scalar : Type u} [field scalar] [inhabited scalar] {f : geom1d_frame} {sp : geom1d_space f} : has_coe (position1d sp) (position1d_expr sp) := ⟨λt, position1d_expr.lit t⟩
+--instance {scalar : Type u} [field scalar] [inhabited scalar] {f : geom1d_frame} {sp : geom1d_space f} : has_coe (displacement1d sp) (displacement1d_expr sp) := ⟨λt, displacement1d_expr.lit t⟩
+--instance {scalar : Type u} [field scalar] [inhabited scalar] : has_coe (geom1d_frame) (geom1d_frame_expr scalar) := ⟨λf, geom1d_frame_expr.lit f⟩
+--instance {scalar : Type u} [field scalar] [inhabited scalar] {f : geom1d_frame} : has_coe (geom1d_space f) (geom1d_space_expr scalar) := ⟨λs, geom1d_space_expr.lit s⟩
 
 /-
 class has_lit (t1 : Type 0) (t2 : Type 1) :=
   (cast : t1 → t2)
 notation `|`lit`|` := has_lit.cast lit
-instance position_lit {f : geom1d_frame_expr} {sp : geom1d_space_expr f } : has_lit (position sp.value) (position_expr sp) :=
-  ⟨λt, position_expr.lit t⟩
-instance displacement_lit {f : geom1d_frame_expr} {sp : geom1d_space_expr f } : has_lit (displacement sp.value) (displacement_expr sp) :=
-  ⟨λd, displacement_expr.lit d⟩
-instance position_space_lit {f : geom1d_frame_expr} : has_lit (spc scalar f.value) (geom1d_space_expr f) :=
+instance position1d_lit {f : geom1d_frame_expr} {sp : geom1d_space_expr f } : has_lit (position1d sp.value) (position1d_expr sp) :=
+  ⟨λt, position1d_expr.lit t⟩
+instance displacement1d_lit {f : geom1d_frame_expr} {sp : geom1d_space_expr f } : has_lit (displacement1d sp.value) (displacement1d_expr sp) :=
+  ⟨λd, displacement1d_expr.lit d⟩
+instance position1d_space_lit {f : geom1d_frame_expr} : has_lit (geom1d_space f.value) (geom1d_space_expr f) :=
   ⟨λs, geom1d_space_expr.lit s⟩
-instance position_frame_lit : has_lit (fm scalar LENGTH) (geom1d_frame_expr) :=
+instance position1d_frame_lit : has_lit (geom1d_frame) (geom1d_frame_expr) :=
   ⟨λf, geom1d_frame_expr.lit f⟩
 -/
 
-class position_has_lit {f : geom1d_frame_expr} (sp : geom1d_space_expr f) := 
-  (cast : position sp.value → position_expr sp)
-notation `|`tlit`|` := position_has_lit.cast tlit
+class position1d_has_lit {f : geom1d_frame_expr} (sp : geom1d_space_expr f) := 
+  (cast : position1d sp.value → position1d_expr sp)
+notation `|`tlit`|` := position1d_has_lit.cast tlit
 
-instance position_lit {f : geom1d_frame_expr} (sp : geom1d_space_expr f) : position_has_lit  sp := 
-  ⟨λt : position sp.value, position_expr.lit t⟩
+instance position1d_lit {f : geom1d_frame_expr} (sp : geom1d_space_expr f) : position1d_has_lit  sp := 
+  ⟨λt : position1d sp.value, position1d_expr.lit t⟩
 
-class displacement_has_lit {f : geom1d_frame_expr} (sp : geom1d_space_expr f) := 
-  (cast : displacement sp.value → displacement_expr sp)
-notation `|`tlit`|` := displacement_has_lit.cast tlit
+class displacement1d_has_lit {f : geom1d_frame_expr} (sp : geom1d_space_expr f) := 
+  (cast : displacement1d sp.value → displacement1d_expr sp)
+notation `|`tlit`|` := displacement1d_has_lit.cast tlit
 
-instance displacement_lit {f : geom1d_frame_expr} (sp : geom1d_space_expr f) : displacement_has_lit  sp := 
-  ⟨λt : displacement sp.value, displacement_expr.lit t⟩
+instance displacement1d_lit {f : geom1d_frame_expr} (sp : geom1d_space_expr f) : displacement1d_has_lit  sp := 
+  ⟨λt : displacement1d sp.value, displacement1d_expr.lit t⟩
 
-class position_frame_has_lit := 
-  (cast : fm scalar LENGTH → geom1d_frame_expr)
-notation `|`flit`|` := position_frame_has_lit.cast flit
+class position1d_frame_has_lit := 
+  (cast : geom1d_frame → geom1d_frame_expr)
+notation `|`flit`|` := position1d_frame_has_lit.cast flit
 
-instance position_frame_lit : position_frame_has_lit := 
+instance position1d_frame_lit : position1d_frame_has_lit := 
   ⟨λf, geom1d_frame_expr.lit f⟩
 
-class position_space_has_lit (f : geom1d_frame_expr ) := 
-  (cast : spc scalar f.value  → geom1d_space_expr f)
-notation `|`slit`|` := position_space_has_lit.cast slit
+class position1d_space_has_lit (f : geom1d_frame_expr ) := 
+  (cast : geom1d_space f.value  → geom1d_space_expr f)
+notation `|`slit`|` := position1d_space_has_lit.cast slit
 
-instance position_space_lit {f : geom1d_frame_expr} : position_space_has_lit f := 
+instance position1d_space_lit {f : geom1d_frame_expr} : position1d_space_has_lit f := 
   ⟨λs, geom1d_space_expr.lit s⟩
 
 
@@ -341,8 +342,8 @@ Analogous methods provided at math layer
 #check mk_frame
 
 #check mk_frame
-def mk_geom1d_frame_expr {f : geom1d_frame_expr} {sp : geom1d_space_expr f} (o : position_expr sp) (b : displacement_expr sp) : geom1d_frame_expr :=
-  [(mk_frame o.value.to_point b.value.to_vectr)]
+def mk_geom1d_frame_expr {f : geom1d_frame_expr} {sp : geom1d_space_expr f} (o : position1d_expr sp) (b : displacement1d_expr sp) : geom1d_frame_expr :=
+  |(mk_geom1d_frame o.value b.value)|
 /-
 4/7
 WRITE THIS FUNCTION LATER. 
@@ -355,27 +356,27 @@ def mk_geom1d_space_expr (f : geom1d_frame_expr) : geom1d_space_expr f :=
 
 
 
-def add_dur_expr_dur_expr (v1 v2 : displacement_expr sp) : displacement_expr sp := 
-  displacement_expr.add_dur_dur v1 v2
+def add_dur_expr_dur_expr (v1 v2 : displacement1d_expr sp) : displacement1d_expr sp := 
+  displacement1d_expr.add_dur_dur v1 v2
 
-def smul_dur_expr (k : scalar_expr) (v : displacement_expr sp) : displacement_expr sp := 
-    displacement_expr.smul_dur k v
+def smul_dur_expr (k : scalar_expr) (v : displacement1d_expr sp) : displacement1d_expr sp := 
+    displacement1d_expr.smul_dur k v
 
-def neg_dur_expr (v : displacement_expr sp) : displacement_expr sp := 
-    displacement_expr.neg_dur v
+def neg_dur_expr (v : displacement1d_expr sp) : displacement1d_expr sp := 
+    displacement1d_expr.neg_dur v
 
-def sub_dur_expr_dur_expr (v1 v2 : displacement_expr sp) : displacement_expr sp :=    -- v1-v2
-    displacement_expr.sub_dur_dur v1 v2
+def sub_dur_expr_dur_expr (v1 v2 : displacement1d_expr sp) : displacement1d_expr sp :=    -- v1-v2
+    displacement1d_expr.sub_dur_dur v1 v2
 
 -- See unframed file for template for proving vector_space
-instance has_one_dur_expr : has_one (displacement_expr sp) := ⟨displacement_expr.one⟩
+instance has_one_dur_expr : has_one (displacement1d_expr sp) := ⟨displacement1d_expr.one⟩
 
-instance has_add_dur_expr : has_add (displacement_expr sp) := ⟨ add_dur_expr_dur_expr ⟩
+instance has_add_dur_expr : has_add (displacement1d_expr sp) := ⟨ add_dur_expr_dur_expr ⟩
 
 /-
 THIS IS UNPROVABLE
 -/
-lemma add_assoc_dur_expr : ∀ a b c : displacement_expr sp, a + b + c = a + (b + c) :=
+lemma add_assoc_dur_expr : ∀ a b c : displacement1d_expr sp, a + b + c = a + (b + c) :=
 begin
     intros,
     cases a,
@@ -411,14 +412,14 @@ begin
     }
 end
 
-instance add_semigroup_dur_expr : add_semigroup (displacement_expr sp) := ⟨ add_dur_expr_dur_expr, add_assoc_dur_expr⟩ 
+instance add_semigroup_dur_expr : add_semigroup (displacement1d_expr sp) := ⟨ add_dur_expr_dur_expr, add_assoc_dur_expr⟩ 
 
-def dur_expr_zero : displacement_expr sp := displacement_expr.zero--displacement_expr.lit (mk_displacement sp.value 0)
-instance has_zero_dur_expr : has_zero (displacement_expr sp) := ⟨dur_expr_zero⟩
+def dur_expr_zero : displacement1d_expr sp := displacement1d_expr.zero--displacement1d_expr.lit (mk_displacement1d sp.value 0)
+instance has_zero_dur_expr : has_zero (displacement1d_expr sp) := ⟨dur_expr_zero⟩
 
-lemma zero_add_dur_expr : ∀ a : displacement_expr sp, 0 + a = a := sorry
-lemma add_zero_dur_expr : ∀ a : displacement_expr sp, a + 0 = a := sorry
-instance add_monoid_dur_expr : add_monoid (displacement_expr sp) := ⟨ 
+lemma zero_add_dur_expr : ∀ a : displacement1d_expr sp, 0 + a = a := sorry
+lemma add_zero_dur_expr : ∀ a : displacement1d_expr sp, a + 0 = a := sorry
+instance add_monoid_dur_expr : add_monoid (displacement1d_expr sp) := ⟨ 
     -- add_semigroup
     add_dur_expr_dur_expr, 
     add_assoc_dur_expr, 
@@ -429,10 +430,10 @@ instance add_monoid_dur_expr : add_monoid (displacement_expr sp) := ⟨
     add_zero_dur_expr
 ⟩
 
-instance has_neg_dur_expr : has_neg (displacement_expr sp) := ⟨neg_dur_expr⟩
-instance has_sub_dur_expr : has_sub (displacement_expr sp) := ⟨ sub_dur_expr_dur_expr⟩ 
-lemma sub_eq_add_neg_dur_expr : ∀ a b : displacement_expr sp, a - b = a + -b := sorry
-instance sub_neg_monoid_dur_expr : sub_neg_monoid (displacement_expr sp) := ⟨ 
+instance has_neg_dur_expr : has_neg (displacement1d_expr sp) := ⟨neg_dur_expr⟩
+instance has_sub_dur_expr : has_sub (displacement1d_expr sp) := ⟨ sub_dur_expr_dur_expr⟩ 
+lemma sub_eq_add_neg_dur_expr : ∀ a b : displacement1d_expr sp, a - b = a + -b := sorry
+instance sub_neg_monoid_dur_expr : sub_neg_monoid (displacement1d_expr sp) := ⟨ 
     add_dur_expr_dur_expr, add_assoc_dur_expr, dur_expr_zero, 
     zero_add_dur_expr, 
     add_zero_dur_expr, -- add_monoid
@@ -441,8 +442,8 @@ instance sub_neg_monoid_dur_expr : sub_neg_monoid (displacement_expr sp) := ⟨
     sub_eq_add_neg_dur_expr,                                                       -- new
 ⟩ 
 
-lemma add_left_neg_dur_expr : ∀ a : displacement_expr sp, -a + a = 0 := sorry
-instance : add_group (displacement_expr sp) := ⟨
+lemma add_left_neg_dur_expr : ∀ a : displacement1d_expr sp, -a + a = 0 := sorry
+instance : add_group (displacement1d_expr sp) := ⟨
     -- sub_neg_monoid
     add_dur_expr_dur_expr, add_assoc_dur_expr, dur_expr_zero, zero_add_dur_expr, add_zero_dur_expr, -- add_monoid
     neg_dur_expr,                                                                  -- has_neg
@@ -452,15 +453,15 @@ instance : add_group (displacement_expr sp) := ⟨
     add_left_neg_dur_expr,
 ⟩ 
 
-lemma add_comm_dur_expr : ∀ a b : displacement_expr sp, a + b = b + a := sorry
-instance add_comm_semigroup_dur_expr : add_comm_semigroup (displacement_expr sp) := ⟨
+lemma add_comm_dur_expr : ∀ a b : displacement1d_expr sp, a + b = b + a := sorry
+instance add_comm_semigroup_dur_expr : add_comm_semigroup (displacement1d_expr sp) := ⟨
     -- add_semigroup
     add_dur_expr_dur_expr, 
     add_assoc_dur_expr,
     add_comm_dur_expr,
 ⟩
 
-instance add_comm_monoid_dur_expr : add_comm_monoid (displacement_expr sp) := ⟨
+instance add_comm_monoid_dur_expr : add_comm_monoid (displacement1d_expr sp) := ⟨
 -- add_monoid
     -- add_semigroup
     add_dur_expr_dur_expr, 
@@ -474,33 +475,33 @@ instance add_comm_monoid_dur_expr : add_comm_monoid (displacement_expr sp) := �
     add_comm_dur_expr,
 ⟩
 
-instance has_scalar_dur_expr : has_scalar scalar_expr (displacement_expr sp) := ⟨
+instance has_scalar_dur_expr : has_scalar scalar_expr (displacement1d_expr sp) := ⟨
 smul_dur_expr,
 ⟩
 instance : has_one scalar_expr := sorry
 instance : monoid scalar_expr := sorry
 instance : has_zero scalar_expr := sorry
 
-lemma one_smul_dur_expr : ∀ b : displacement_expr sp, (1 : scalar_expr) • b = b := sorry
-lemma mul_smul_dur_expr : ∀ (x y : scalar_expr) (b : displacement_expr sp), (x * y) • b = x • y • b := sorry
-instance mul_action_dur_expr : mul_action scalar_expr (displacement_expr sp) := sorry /-⟨
+lemma one_smul_dur_expr : ∀ b : displacement1d_expr sp, (1 : scalar_expr) • b = b := sorry
+lemma mul_smul_dur_expr : ∀ (x y : scalar_expr) (b : displacement1d_expr sp), (x * y) • b = x • y • b := sorry
+instance mul_action_dur_expr : mul_action scalar_expr (displacement1d_expr sp) := sorry /-⟨
 one_smul_dur_expr,
 mul_smul_dur_expr,
 ⟩ -/
 
-lemma smul_add_dur_expr : ∀(r : scalar_expr) (x y : displacement_expr sp), r • (x + y) = r • x + r • y := sorry
-lemma smul_zero_dur_expr : ∀(r : scalar_expr), r • (0 : displacement_expr sp) = 0 := sorry
-instance distrib_mul_action_K_dur_exprKx : distrib_mul_action scalar_expr (displacement_expr sp) := ⟨
+lemma smul_add_dur_expr : ∀(r : scalar_expr) (x y : displacement1d_expr sp), r • (x + y) = r • x + r • y := sorry
+lemma smul_zero_dur_expr : ∀(r : scalar_expr), r • (0 : displacement1d_expr sp) = 0 := sorry
+instance distrib_mul_action_K_dur_exprKx : distrib_mul_action scalar_expr (displacement1d_expr sp) := ⟨
 smul_add_dur_expr,
 smul_zero_dur_expr,
 ⟩ 
 
 -- renaming vs template due to clash with name "s" for prevailing variable
-lemma add_smul_dur_expr : ∀ (a b : scalar_expr) (x : displacement_expr sp), (a + b) • x = a • x + b • x := sorry
-lemma zero_smul_dur_expr : ∀ (x : displacement_expr sp), (0 : scalar_expr) • x = 0 := sorry
-instance semimodule_K_displacementK : semimodule scalar_expr (displacement_expr sp) := ⟨ add_smul_dur_expr, zero_smul_dur_expr ⟩ 
+lemma add_smul_dur_expr : ∀ (a b : scalar_expr) (x : displacement1d_expr sp), (a + b) • x = a • x + b • x := sorry
+lemma zero_smul_dur_expr : ∀ (x : displacement1d_expr sp), (0 : scalar_expr) • x = 0 := sorry
+instance semimodule_K_displacement1dK : semimodule scalar_expr (displacement1d_expr sp) := ⟨ add_smul_dur_expr, zero_smul_dur_expr ⟩ 
 
-instance add_comm_group_dur_expr : add_comm_group (displacement_expr sp) := ⟨
+instance add_comm_group_dur_expr : add_comm_group (displacement1d_expr sp) := ⟨
 -- add_group
     add_dur_expr_dur_expr, add_assoc_dur_expr, dur_expr_zero, zero_add_dur_expr, add_zero_dur_expr, -- add_monoid
     neg_dur_expr,                                                                  -- has_neg
@@ -512,7 +513,7 @@ instance add_comm_group_dur_expr : add_comm_group (displacement_expr sp) := ⟨
 ⟩
 
 
-instance : vector_space scalar (displacement_expr sp) := sorry
+instance : vector_space scalar (displacement1d_expr sp) := sorry
 
 
 /-
@@ -525,56 +526,56 @@ instance : vector_space scalar (displacement_expr sp) := sorry
 /-
 Affine operations
 -/
-instance : has_add (displacement_expr sp) := ⟨add_dur_expr_dur_expr⟩
-instance : has_zero (displacement_expr sp) := ⟨dur_expr_zero⟩
-instance : has_neg (displacement_expr sp) := ⟨neg_dur_expr⟩
+instance : has_add (displacement1d_expr sp) := ⟨add_dur_expr_dur_expr⟩
+instance : has_zero (displacement1d_expr sp) := ⟨dur_expr_zero⟩
+instance : has_neg (displacement1d_expr sp) := ⟨neg_dur_expr⟩
 
 /-
 Lemmas needed to implement affine space API
 -/
 
-def sub_position_expr_position_expr {f : geom1d_frame_expr} {sp : geom1d_space_expr f}  (p1 p2 : position_expr sp) : displacement_expr sp := 
-    displacement_expr.sub_position_position p1 p2
-def add_position_expr_dur_expr {f : geom1d_frame_expr} {sp : geom1d_space_expr f}  (p : position_expr sp) (v : displacement_expr sp) : position_expr sp := 
-    position_expr.add_dur_position v p
-def add_dur_expr_position_expr {f : geom1d_frame_expr} {sp : geom1d_space_expr f}  (v : displacement_expr sp) (p : position_expr sp) : position_expr sp := 
-    position_expr.add_dur_position v p
+def sub_position1d_expr_position1d_expr {f : geom1d_frame_expr} {sp : geom1d_space_expr f}  (p1 p2 : position1d_expr sp) : displacement1d_expr sp := 
+    displacement1d_expr.sub_position1d_position1d p1 p2
+def add_position1d_expr_dur_expr {f : geom1d_frame_expr} {sp : geom1d_space_expr f}  (p : position1d_expr sp) (v : displacement1d_expr sp) : position1d_expr sp := 
+    position1d_expr.add_dur_position1d v p
+def add_dur_expr_position1d_expr {f : geom1d_frame_expr} {sp : geom1d_space_expr f}  (v : displacement1d_expr sp) (p : position1d_expr sp) : position1d_expr sp := 
+    position1d_expr.add_dur_position1d v p
 
-def aff_dur_expr_group_action {f : geom1d_frame_expr} {sp : geom1d_space_expr f} : displacement_expr sp → position_expr sp → position_expr sp := add_dur_expr_position_expr
-instance {f : geom1d_frame_expr} {sp : geom1d_space_expr f} : has_vadd (displacement_expr sp) (position_expr sp) := ⟨λd, λt, position_expr.add_dur_position d t⟩
+def aff_dur_expr_group_action {f : geom1d_frame_expr} {sp : geom1d_space_expr f} : displacement1d_expr sp → position1d_expr sp → position1d_expr sp := add_dur_expr_position1d_expr
+instance {f : geom1d_frame_expr} {sp : geom1d_space_expr f} : has_vadd (displacement1d_expr sp) (position1d_expr sp) := ⟨λd, λt, position1d_expr.add_dur_position1d d t⟩
 
 def spf : geom1d_space_expr [geom1d_std_frame] := [(geom1d_std_space)]
 
-variables (d d2 : displacement_expr spf) (t : position_expr spf) (df : displacement_expr spf)
+variables (d d2 : displacement1d_expr spf) (t : position1d_expr spf) (df : displacement1d_expr spf)
 
-#check position_expr.add_dur_position d t
+#check position1d_expr.add_dur_position1d d t
 
-lemma zero_dur_expr_vadd'_a1 {f : geom1d_frame_expr} {sp : geom1d_space_expr f} : ∀ p : position_expr sp, (0 : displacement_expr sp) +ᵥ p = p := sorry
-lemma dur_expr_add_assoc'_a1 : ∀ (g1 g2 : displacement_expr sp) (p : position_expr sp), g1 +ᵥ (g2 +ᵥ p) = (g1 + g2) +ᵥ p := sorry
-instance dur_expr_add_action: add_action (displacement_expr sp) (position_expr sp) := 
+lemma zero_dur_expr_vadd'_a1 {f : geom1d_frame_expr} {sp : geom1d_space_expr f} : ∀ p : position1d_expr sp, (0 : displacement1d_expr sp) +ᵥ p = p := sorry
+lemma dur_expr_add_assoc'_a1 : ∀ (g1 g2 : displacement1d_expr sp) (p : position1d_expr sp), g1 +ᵥ (g2 +ᵥ p) = (g1 + g2) +ᵥ p := sorry
+instance dur_expr_add_action: add_action (displacement1d_expr sp) (position1d_expr sp) := 
 ⟨ aff_dur_expr_group_action, zero_dur_expr_vadd'_a1, dur_expr_add_assoc'_a1 ⟩ 
 
-def aff_position_expr_group_sub : position_expr sp → position_expr sp → displacement_expr sp := sub_position_expr_position_expr
-instance position_expr_has_vsub : has_vsub (displacement_expr sp) (position_expr sp) := ⟨ aff_position_expr_group_sub ⟩ 
+def aff_position1d_expr_group_sub : position1d_expr sp → position1d_expr sp → displacement1d_expr sp := sub_position1d_expr_position1d_expr
+instance position1d_expr_has_vsub : has_vsub (displacement1d_expr sp) (position1d_expr sp) := ⟨ aff_position1d_expr_group_sub ⟩ 
 
 
-instance : nonempty (position_expr sp) := ⟨position_expr.lit (mk_position sp.value  0)⟩
+instance : nonempty (position1d_expr sp) := ⟨position1d_expr.lit (mk_position1d sp.value  0)⟩
 
-lemma position_expr_vsub_vadd_a1 : ∀ (p1 p2 : (position_expr sp)), (p1 -ᵥ p2) +ᵥ p2 = p1 := sorry
-lemma position_expr_vadd_vsub_a1 : ∀ (g : displacement_expr sp) (p : position_expr sp), g +ᵥ p -ᵥ p = g := sorry
-instance aff_position_expr_torsor : add_torsor (displacement_expr sp) (position_expr sp) := --affine space! 
+lemma position1d_expr_vsub_vadd_a1 : ∀ (p1 p2 : (position1d_expr sp)), (p1 -ᵥ p2) +ᵥ p2 = p1 := sorry
+lemma position1d_expr_vadd_vsub_a1 : ∀ (g : displacement1d_expr sp) (p : position1d_expr sp), g +ᵥ p -ᵥ p = g := sorry
+instance aff_position1d_expr_torsor : add_torsor (displacement1d_expr sp) (position1d_expr sp) := --affine space! 
 ⟨ 
     aff_dur_expr_group_action,
     zero_dur_expr_vadd'_a1,    -- add_action
     dur_expr_add_assoc'_a1,   -- add_action
-    aff_position_expr_group_sub,    -- has_vsub
-    position_expr_vsub_vadd_a1,     -- add_torsor
-    position_expr_vadd_vsub_a1,     -- add_torsor
+    aff_position1d_expr_group_sub,    -- has_vsub
+    position1d_expr_vsub_vadd_a1,     -- add_torsor
+    position1d_expr_vadd_vsub_a1,     -- add_torsor
 ⟩
 
-notation t+ᵥv := add_dur_expr_position_expr v t
+notation t+ᵥv := add_dur_expr_position1d_expr v t
 notation d•k :=  smul_dur_expr k d
-notation tr⬝d := displacement_expr.apply_displacement_lit tr d
-notation tr⬝t := position_expr.apply_position_lit tr t
+notation tr⬝d := displacement1d_expr.apply_displacement1d_lit tr d
+notation tr⬝t := position1d_expr.apply_position1d_lit tr t
 
-end lang.position
+end lang.geom1d
